examples/QueryStructure/Messages.v
@@ -75,10 +75,48 @@ Proof.
 
   GenerateIndexesForAll matchInclusionClause ltac:(fun l => make simple indexes using l).
 
+
+    hone method "AddMessage".
+  {
+    Implement_Insert_Checks.
+    Focused_refine_Query.
+    {
+      (* Step 1: Implement [In] by enumeration. *)
+      implement_In;
+      (* Step 2: Convert where clauses into compositions of filters. *)
+      repeat convert_Where_to_filter.
+      (* Step 3: Do some simplication.*)
+    repeat setoid_rewrite <- filter_and;
+    try setoid_rewrite andb_true_r.
+    (* Step 4: Move filters to the outermost [Join_Comp_Lists] to which *)
+    (* they can be applied. *)
+    repeat setoid_rewrite Join_Filtered_Comp_Lists_id;
+    distribute_filters_to_joins.
+    (* Step 5: Convert filter function on topmost [Join_Filtered_Comp_Lists] to an
+               equivalent search term matching function.  *)
+    implement_filters_with_find
+      ltac:(find_simple_search_term
+              InclusionIndexUse createLastInclusionTerm createEarlyInclusionTerm)
+             ltac:(find_simple_search_term_dep
+                     InclusionIndexUse_dep createLastInclusionTerm_dep createEarlyInclusionTerm_dep).
+  |
+  ].
+
+InclusionIndexUse createLastInclusionTerm createEarlyInclusionTerm
+      InclusionIndexUse_dep createLastInclusionTerm_dep createEarlyInclusionTerm_dep.
+
+    implement_Query.
+    simpl; simplify with monad laws.
+    setoid_rewrite refineEquiv_swap_bind.
+    implement_Insert_branches.
+
+    cleanup_Count.
+    finish honing.
+  }
   hone method "RelevantMessages".
   {
     implement_Query InclusionIndexUse createLastInclusionTerm createEarlyInclusionTerm
-      InclusionIndexUse_dep createLastInclusionTerm_dep createEarlyInclusionTerm_dep.  
+      InclusionIndexUse_dep createLastInclusionTerm_dep createEarlyInclusionTerm_dep.
     (* Do some more simplication using the monad laws. *)
     simpl; simplify with monad laws.
     (* Satisfied with the query, we now implement the new data
